zoo_saturn/inf_mpmc_queue_1: Rewrite.

theories/zoo_saturn/inf_mpmc_queue_1.v
@@ -30,8 +30,7 @@ From zoo Require Import
   options.
 
 Implicit Types front back : nat.
-Implicit Types l : location.
-Implicit Types t v : val.
+Implicit Types v : val.
 Implicit Types vs hist : list val.
 Implicit Types slot : optional val.
 Implicit Types slots : nat → optional val.
@@ -83,445 +82,865 @@ Proof.
   solve_inG.
 Qed.
 
+Module base.
+  Section inf_mpmc_queue_1_G.
+    Context `{inf_mpmc_queue_1_G : InfMpmcQueue1G Σ}.
+
+    Implicit Types t : location.
+    Implicit Types Ψ : val → iProp Σ.
+
+    Record inf_mpmc_queue_1_name := {
+      inf_mpmc_queue_1_name_data : val ;
+      inf_mpmc_queue_1_name_inv : namespace ;
+      inf_mpmc_queue_1_name_model : gname ;
+      inf_mpmc_queue_1_name_history : gname ;
+      inf_mpmc_queue_1_name_consumers : gname ;
+      inf_mpmc_queue_1_name_tokens : gname ;
+    }.
+    Implicit Types γ : inf_mpmc_queue_1_name.
+
+    #[global] Instance inf_mpmc_queue_1_name_eq_dec : EqDecision inf_mpmc_queue_1_name :=
+      ltac:(solve_decision).
+    #[global] Instance inf_mpmc_queue_1_name_countable :
+      Countable inf_mpmc_queue_1_name.
+    Proof.
+      solve_countable.
+    Qed.
+
+    #[local] Definition model₁' γ_model vs :=
+      twins_twin1 γ_model (DfracOwn 1) vs.
+    #[local] Definition model₁ γ :=
+      model₁' γ.(inf_mpmc_queue_1_name_model).
+    #[local] Definition model₂' γ_model vs :=
+      twins_twin2 γ_model vs.
+    #[local] Definition model₂ γ :=
+      model₂' γ.(inf_mpmc_queue_1_name_model).
+
+    #[local] Definition history_auth' γ_history hist :=
+      mono_list_auth γ_history (DfracOwn 1) hist.
+    #[local] Definition history_auth γ :=
+      history_auth' γ.(inf_mpmc_queue_1_name_history).
+    #[local] Definition history_at γ i v :=
+      mono_list_at γ.(inf_mpmc_queue_1_name_history) i v.
+
+    #[local] Definition consumers_auth' γ_consumers i : iProp Σ :=
+      ∃ ηs,
+      mono_list_auth γ_consumers (DfracOwn 1) ηs ∗
+      ⌜length ηs = i⌝.
+    #[local] Definition consumers_auth γ i :=
+      consumers_auth' γ.(inf_mpmc_queue_1_name_consumers) i.
+    #[local] Instance : CustomIpatFormat "consumers_auth" :=
+      " ( %ηs{} &
+          Hauth{} &
+          %Hηs{}
+        )
+      ".
+    #[local] Definition consumers_at γ i Ψ : iProp Σ :=
+      ∃ η,
+      mono_list_at γ.(inf_mpmc_queue_1_name_consumers) i η ∗
+      saved_pred η Ψ.
+    #[local] Instance : CustomIpatFormat "consumers_at" :=
+      " ( %η{} &
+          Hat{} &
+          HΨ{}
+        )
+      ".
+    #[local] Definition consumers_lb γ i : iProp Σ :=
+      ∃ ηs,
+      ⌜length ηs = i⌝ ∗
+      mono_list_lb γ.(inf_mpmc_queue_1_name_consumers) ηs.
+    #[local] Instance : CustomIpatFormat "consumers_lb" :=
+      " ( %ηs{} &
+          %Hηs{} &
+          Hlb{}
+        )
+      ".
+
+    #[local] Definition tokens_auth' γ_tokens i : iProp Σ :=
+      ∃ ηs,
+      mono_list_auth γ_tokens (DfracOwn 1) ηs ∗
+      ⌜length ηs = i⌝.
+    #[local] Definition tokens_auth γ i :=
+      tokens_auth' γ.(inf_mpmc_queue_1_name_tokens) i.
+    #[local] Instance : CustomIpatFormat "tokens_auth" :=
+      " ( %ηs{} &
+          Hauth{} &
+          %Hηs{}
+        )
+      ".
+    #[local] Definition tokens_pending γ i : iProp Σ :=
+      ∃ η,
+      mono_list_at γ.(inf_mpmc_queue_1_name_tokens) i η ∗
+      oneshot_pending η (DfracOwn 1) ().
+    #[local] Instance : CustomIpatFormat "tokens_pending" :=
+      " ( %η{} &
+          Hat{} &
+          Hpending{}
+        )
+      ".
+    #[local] Definition tokens_done γ i : iProp Σ :=
+      ∃ η,
+      mono_list_at γ.(inf_mpmc_queue_1_name_tokens) i η ∗
+      oneshot_shot η ().
+    #[local] Instance : CustomIpatFormat "tokens_done" :=
+      " ( %η{} &
+          Hat{} &
+          Hshot{}
+        )
+      ".
+
+    #[local] Definition consumer_au γ Ψ : iProp Σ :=
+      AU <{
+        ∃∃ vs,
+        model₁ γ vs
+      }> @ ⊤ ∖ ↑γ.(inf_mpmc_queue_1_name_inv), ∅ <{
+        ∀∀ v vs',
+        ⌜vs = v :: vs'⌝ ∗
+        model₁ γ vs'
+      , COMM
+        Ψ v
+      }>.
+
+    #[local] Definition slot_model γ i slot : iProp Σ :=
+      match slot with
+      | Something v =>
+          history_at γ i v
+      | Anything =>
+          tokens_done γ i
+      | Nothing =>
+          True
+      end.
+    #[local] Definition inv_inner t γ : iProp Σ :=
+      ∃ front back hist slots,
+      t.[front] ↦ #front ∗
+      t.[back] ↦ #back ∗
+      inf_array_model γ.(inf_mpmc_queue_1_name_data) (optional_to_val ∘ slots) ∗
+      history_auth γ hist ∗
+      ⌜length hist = back⌝ ∗
+      model₂ γ (drop front hist) ∗
+      consumers_auth γ front ∗
+      tokens_auth γ (front `max` back) ∗
+      ( [∗ list] i ∈ seq 0 back,
+          tokens_pending γ i
+        ∨ ∃ Ψ,
+          consumers_at γ i Ψ ∗
+          ( tokens_done γ i
+          ∨ ∃ v,
+            history_at γ i v ∗
+            Ψ v
+          )
+      ) ∗
+      ( [∗ list] i ∈ seq back (front - back),
+        ∃ Ψ,
+        consumers_at γ i Ψ ∗
+        consumer_au γ Ψ
+      ) ∗
+      (∀ i, slot_model γ i (slots i)).
+    #[local] Instance : CustomIpatFormat "inv_inner" :=
+      " ( %front{} &
+          %back{} &
+          %hist{} &
+          %slots{} &
+          Ht_front &
+          Ht_back &
+          >Hdata_model &
+          >Hhistory_auth &
+          >%Hhist{} &
+          Hmodel₂ &
+          Hconsumers_auth &
+          Htokens_auth &
+          Hpast &
+          Hwaiters &
+          Hslots
+        )
+      ".
+    Definition inv' t γ : iProp Σ :=
+      t.[data] ↦□ γ.(inf_mpmc_queue_1_name_data) ∗
+      inf_array_inv γ.(inf_mpmc_queue_1_name_data) ∗
+      inv γ.(inf_mpmc_queue_1_name_inv) (inv_inner t γ).
+    #[local] Instance : CustomIpatFormat "inv'" :=
+      " ( #Ht_data &
+          #Hdata_inv &
+          #Hinv
+        )
+      ".
+    Definition inf_mpmc_queue_1_inv t γ ι : iProp Σ :=
+      ⌜ι = γ.(inf_mpmc_queue_1_name_inv)⌝ ∗
+      inv' t γ.
+    #[local] Instance : CustomIpatFormat "inv" :=
+      " ( -> &
+          (:inv')
+        )
+      ".
+
+    Definition inf_mpmc_queue_1_model γ vs : iProp Σ :=
+      model₁ γ vs.
+    #[local] Instance : CustomIpatFormat "model" :=
+      " Hmodel₁{_{}}
+      ".
+
+    #[local] Instance tokens_pending_timeless γ i :
+      Timeless (tokens_pending γ i).
+    Proof.
+      apply _.
+    Qed.
+    #[local] Instance tokens_done_timeless γ i :
+      Timeless (tokens_done γ i).
+    Proof.
+      apply _.
+    Qed.
+    #[local] Instance slot_model_timeless γ i slot :
+      Timeless (slot_model γ i slot).
+    Proof.
+      rewrite /slot_model. apply _.
+    Qed.
+    #[global] Instance inf_mpmc_queue_1_model_timeless γ vs :
+      Timeless (inf_mpmc_queue_1_model γ vs).
+    Proof.
+      apply _.
+    Qed.
+
+    #[local] Instance consumers_at_persistent γ i Ψ :
+      Persistent (consumers_at γ i Ψ).
+    Proof.
+      apply _.
+    Qed.
+    #[local] Instance consumers_lb_persistent γ i :
+      Persistent (consumers_lb γ i).
+    Proof.
+      apply _.
+    Qed.
+    #[local] Instance tokens_done_persistent γ i :
+      Persistent (tokens_done γ i).
+    Proof.
+      apply _.
+    Qed.
+    #[local] Instance slot_model_persistent γ i slot :
+      Persistent (slot_model γ i slot).
+    Proof.
+      rewrite /slot_model. apply _.
+    Qed.
+    #[global] Instance inf_mpmc_queue_1_inv_persistent t γ ι :
+      Persistent (inf_mpmc_queue_1_inv t γ ι).
+    Proof.
+      apply _.
+    Qed.
+
+    #[local] Lemma model_alloc :
+      ⊢ |==>
+        ∃ γ_model,
+        model₁' γ_model [] ∗
+        model₂' γ_model [].
+    Proof.
+      apply twins_alloc'.
+    Qed.
+    #[local] Lemma model₁_exclusive γ vs1 vs2 :
+      model₁ γ vs1 -∗
+      model₁ γ vs2 -∗
+      False.
+    Proof.
+      apply twins_twin1_exclusive.
+    Qed.
+    #[local] Lemma model_agree γ vs1 vs2 :
+      model₁ γ vs1 -∗
+      model₂ γ vs2 -∗
+      ⌜vs1 = vs2⌝.
+    Proof.
+      apply: twins_agree_L.
+    Qed.
+    #[local] Lemma model_update {γ vs1 vs2} vs :
+      model₁ γ vs1 -∗
+      model₂ γ vs2 ==∗
+        model₁ γ vs ∗
+        model₂ γ vs.
+    Proof.
+      apply twins_update.
+    Qed.
+
+    #[local] Lemma history_alloc :
+      ⊢ |==>
+        ∃ γ_history,
+        history_auth' γ_history [].
+    Proof.
+      apply mono_list_alloc.
+    Qed.
+    #[local] Lemma history_at_valid γ hist i v :
+      history_auth γ hist -∗
+      history_at γ i v -∗
+      ⌜hist !! i = Some v⌝.
+    Proof.
+      apply mono_list_at_valid.
+    Qed.
+    #[local] Lemma history_at_agree γ i v1 v2 :
+      history_at γ i v1 -∗
+      history_at γ i v2 -∗
+      ⌜v1 = v2⌝.
+    Proof.
+      apply mono_list_at_agree.
+    Qed.
+    #[local] Lemma history_at_get {γ hist} i v :
+      hist !! i = Some v →
+      history_auth γ hist ⊢
+      history_at γ i v.
+    Proof.
+      apply mono_list_at_get.
+    Qed.
+    #[local] Lemma history_update {γ hist} v :
+      history_auth γ hist ⊢ |==>
+        history_auth γ (hist ++ [v]) ∗
+        history_at γ (length hist) v.
+    Proof.
+      iIntros "Hhistory_auth".
+      iMod (mono_list_update_snoc v with "Hhistory_auth") as "Hhistory_auth".
+      iDestruct (mono_list_at_get with "Hhistory_auth") as "#Hhistory_at".
+      { rewrite list_lookup_middle //. }
+      iSteps.
+    Qed.
+
+    #[local] Lemma consumers_alloc :
+      ⊢ |==>
+        ∃ γ_consumers,
+        consumers_auth' γ_consumers 0.
+    Proof.
+      iMod mono_list_alloc as "(%γ_consumers & Hauth)".
+      iExists _, []. iSteps.
+    Qed.
+    #[local] Lemma consumers_at_valid γ i j Ψ :
+      consumers_auth γ i -∗
+      consumers_at γ j Ψ -∗
+      ⌜j < i⌝.
+    Proof.
+      iIntros "(:consumers_auth) (:consumers_at)".
+      iDestruct (mono_list_at_valid with "Hauth Hat") as %?Hj%lookup_lt_Some.
+      iSteps.
+    Qed.
+    #[local] Lemma consumers_at_agree γ i Ψ1 Ψ2 v :
+      consumers_at γ i Ψ1 -∗
+      ▷ consumers_at γ i Ψ2 -∗
+      ▷ Ψ2 v -∗
+      ▷^2 Ψ1 v.
+    Proof.
+      iIntros "(:consumers_at =1) (:consumers_at =2) HΨ !>".
+      iDestruct (mono_list_at_agree with "Hat1 Hat2") as %<-.
+      iDestruct (saved_pred_agree v with "HΨ1 HΨ2") as "Heq".
+      iModIntro. iRewrite "Heq". iSteps.
+    Qed.
+    #[local] Lemma consumers_lb_valid γ i j :
+      consumers_auth γ i -∗
+      consumers_lb γ j -∗
+      ⌜j ≤ i⌝.
+    Proof.
+      iIntros "(:consumers_auth =1) (:consumers_lb =2)".
+      iDestruct (mono_list_lb_valid with "Hauth1 Hlb2") as %?%prefix_length.
+      iSteps.
+    Qed.
+    #[local] Lemma consumers_lb_get γ i :
+      consumers_auth γ i ⊢
+      consumers_lb γ i.
+    Proof.
+      iIntros "(:consumers_auth)".
+      iDestruct (mono_list_lb_get with "Hauth") as "Hlb".
+      iSteps.
+    Qed.
+    #[local] Lemma consumers_update {γ i} Ψ :
+      consumers_auth γ i ⊢ |==>
+        consumers_auth γ (S i) ∗
+        consumers_at γ i Ψ.
+    Proof.
+      iIntros "(:consumers_auth)".
+      iMod (saved_pred_alloc Ψ) as "(%η & HΨ)".
+      iMod (mono_list_update_snoc with "Hauth") as "Hauth".
+      iDestruct (mono_list_at_get with "Hauth") as "#Hat".
+      { rewrite list_lookup_middle //. }
+      iFrame. simpl_length. iSteps.
+    Qed.
+    Opaque consumers_auth'.
+    Opaque consumers_at.
+    Opaque consumers_lb.
+
+    #[local] Lemma tokens_alloc :
+      ⊢ |==>
+        ∃ γ_tokens,
+        tokens_auth' γ_tokens 0.
+    Proof.
+      iMod mono_list_alloc as "(%γ_tokens & Hauth)".
+      iExists _, []. iSteps.
+    Qed.
+    #[local] Lemma tokens_pending_exclusive γ i :
+      tokens_pending γ i -∗
+      tokens_pending γ i -∗
+      False.
+    Proof.
+      iIntros "(:tokens_pending =1) (:tokens_pending =2)".
+      iDestruct (mono_list_at_agree with "Hat1 Hat2") as %<-.
+      iApply (oneshot_pending_exclusive with "Hpending1 Hpending2").
+    Qed.
+    #[local] Lemma tokens_pending_done γ i :
+      tokens_pending γ i -∗
+      tokens_done γ i -∗
+      False.
+    Proof.
+      iIntros "(:tokens_pending =1) (:tokens_done =2)".
+      iDestruct (mono_list_at_agree with "Hat1 Hat2") as %<-.
+      iApply (oneshot_pending_shot with "Hpending1 Hshot2").
+    Qed.
+    #[local] Lemma tokens_update {γ} i :
+      tokens_auth γ i ⊢ |==>
+        tokens_auth γ (S i) ∗
+        tokens_pending γ i.
+    Proof.
+      iIntros "(:tokens_auth)".
+      iMod oneshot_alloc as "(%η & Hpending)".
+      iMod (mono_list_update_snoc with "Hauth") as "Hauth".
+      iDestruct (mono_list_at_get with "Hauth") as "#Hat".
+      { rewrite list_lookup_middle //. }
+      iFrame. simpl_length. iSteps.
+    Qed.
+    #[local] Lemma tokens_pending_update γ i :
+      tokens_pending γ i ⊢ |==>
+      tokens_done γ i.
+    Proof.
+      iIntros "(:tokens_pending)".
+      iMod (oneshot_update_shot with "Hpending") as "Hshot".
+      iSteps.
+    Qed.
+    Opaque tokens_auth'.
+    Opaque tokens_pending.
+    Opaque tokens_done.
+
+    Lemma inf_mpmc_queue_1_model_exclusive γ vs1 vs2 :
+      inf_mpmc_queue_1_model γ vs1 -∗
+      inf_mpmc_queue_1_model γ vs2 -∗
+      False.
+    Proof.
+      iIntros "(:model =1) (:model =2)".
+      iApply (model₁_exclusive with "Hmodel₁_1 Hmodel₁_2").
+    Qed.
+
+    Lemma inf_mpmc_queue_1_create_spec ι :
+      {{{
+        True
+      }}}
+        inf_mpmc_queue_1_create ()
+      {{{ t γ,
+        RET #t;
+        meta_token t ⊤ ∗
+        inf_mpmc_queue_1_inv t γ ι ∗
+        inf_mpmc_queue_1_model γ []
+      }}}.
+    Proof.
+      iIntros "%Φ _ HΦ".
+
+      wp_rec.
+      wp_apply (inf_array_create_spec with "[//]") as (data) "(#Hdata_inv & Hdata_model)".
+      wp_block t as "Hmeta" "(Ht_data & Ht_front & Ht_back & _)".
+      iMod (pointsto_persist with "Ht_data") as "#Ht_data".
+
+      iMod model_alloc as "(%γ_model & Hmodel₁ & Hmodel₂)".
+      iMod history_alloc as "(%γ_history & Hhistory_auth)".
+      iMod consumers_alloc as "(%γ_consumers & Hconsumers_auth)".
+      iMod tokens_alloc as "(%γ_tokens & Htokens_auth)".
+
+      pose γ := {|
+        inf_mpmc_queue_1_name_data := data ;
+        inf_mpmc_queue_1_name_inv := ι ;
+        inf_mpmc_queue_1_name_model := γ_model ;
+        inf_mpmc_queue_1_name_history := γ_history ;
+        inf_mpmc_queue_1_name_consumers := γ_consumers ;
+        inf_mpmc_queue_1_name_tokens := γ_tokens ;
+      |}.
+
+      iApply ("HΦ" $! t γ).
+      iFrameSteps. iExists (λ _, Nothing). iSteps.
+    Qed.
+
+    Lemma inf_mpmc_queue_1_size_spec t γ ι :
+      <<<
+        inf_mpmc_queue_1_inv t γ ι
+      | ∀∀ vs,
+        inf_mpmc_queue_1_model γ vs
+      >>>
+        inf_mpmc_queue_1_size #t @ ↑ι
+      <<<
+        inf_mpmc_queue_1_model γ vs
+      | RET #(length vs);
+        True
+      >>>.
+    Proof.
+      iIntros "%Φ (:inv) HΦ".
+
+      iLöb as "HLöb".
+
+      wp_rec.
+
+      wp_bind (_.{front})%E.
+      iInv "Hinv" as "(:inv_inner =1)".
+      wp_load.
+      iDestruct (consumers_lb_get with "Hconsumers_auth") as "#Hconsumers_lb1".
+      iSplitR "HΦ". { iFrameSteps. }
+      iIntros "!> {%}".
+
+      wp_smart_apply (typed_prophet1_wp_proph prophet with "[//]") as (pid proph) "Hproph".
+      wp_pures.
+
+      wp_bind (_.{back})%E.
+      iInv "Hinv" as "(:inv_inner =2)".
+      wp_load.
+      destruct_decide (proph = front1) as -> | Hproph.
+
+      - destruct_decide (front2 = front1) as -> | ?.
+
+        + iMod "HΦ" as "(%vs & (:model) & _ & HΦ)".
+          iDestruct (model_agree with "Hmodel₁ Hmodel₂") as %->.
+          iMod ("HΦ" with "Hmodel₁ [//]") as "HΦ".
+
+          iSplitR "Hproph HΦ". { iFrameSteps. }
+          iModIntro. clear- Hhist2.
+
+          wp_pures.
+
+          wp_bind (_.{front})%E.
+          iInv "Hinv" as "(:inv_inner =3)".
+          wp_load.
+          iSplitR "Hproph HΦ". { iFrameSteps. }
+          iModIntro. clear- Hhist2.
+
+          wp_smart_apply (typed_prophet1_wp_resolve with "Hproph"); [done.. |].
+          iSteps.
+          rewrite length_drop Hhist2 Z2Nat.inj_sub; first lia.
+          rewrite !Nat2Z.id //.
+
+        + iDestruct (consumers_lb_valid with "Hconsumers_auth Hconsumers_lb1") as %?.
+          iDestruct (consumers_lb_get with "Hconsumers_auth") as "#Hconsumers_lb2".
+          iSplitR "Hproph HΦ". { iFrameSteps. }
+          iModIntro.
+
+          wp_pures.
+
+          wp_bind (_.{front})%E.
+          iInv "Hinv" as "(:inv_inner =3)".
+          wp_load.
+          iDestruct (consumers_lb_valid with "Hconsumers_auth Hconsumers_lb2") as %?.
+          iSplitR "Hproph HΦ". { iFrameSteps. }
+          iModIntro.
+
+          wp_smart_apply (typed_prophet1_wp_resolve with "Hproph"); [done.. |].
+          iSteps.
+
+      - iSplitR "Hproph HΦ". { iFrameSteps. }
+        iModIntro. clear- Hproph.
+
+        wp_pures.
+
+        wp_bind (_.{front})%E.
+        iInv "Hinv" as "(:inv_inner =3)".
+        wp_load.
+        iSplitR "Hproph HΦ". { iFrameSteps. }
+        iModIntro. clear- Hproph.
+
+        wp_smart_apply (typed_prophet1_wp_resolve with "Hproph"); [done.. |].
+        iSteps.
+    Qed.
+
+    Lemma inf_mpmc_queue_1_is_empty_spec t γ ι :
+      <<<
+        inf_mpmc_queue_1_inv t γ ι
+      | ∀∀ vs,
+        inf_mpmc_queue_1_model γ vs
+      >>>
+        inf_mpmc_queue_1_is_empty #t @ ↑ι
+      <<<
+        inf_mpmc_queue_1_model γ vs
+      | RET #(bool_decide (vs = []%list));
+        True
+      >>>.
+    Proof.
+      iIntros "%Φ #Hinv HΦ".
+
+      wp_rec.
+
+      awp_apply (inf_mpmc_queue_1_size_spec with "Hinv").
+      iApply (aacc_aupd_commit with "HΦ"); first done. iIntros "%vs Hmodel".
+      iAaccIntro with "Hmodel"; iSteps.
+      destruct vs; iSteps.
+    Qed.
+
+    Lemma inf_mpmc_queue_1_push_spec t γ ι v :
+      <<<
+        inf_mpmc_queue_1_inv t γ ι
+      | ∀∀ vs,
+        inf_mpmc_queue_1_model γ vs
+      >>>
+        inf_mpmc_queue_1_push #t v @ ↑ι
+      <<<
+        inf_mpmc_queue_1_model γ (vs ++ [v])
+      | RET ();
+        True
+      >>>.
+    Proof.
+      iIntros "%Φ (:inv) HΦ".
+
+      wp_rec. wp_pures.
+
+      wp_bind (FAA _ _).
+      wp_apply (wp_wand (λ res,
+        ∃ back,
+        ⌜res = #back⌝ ∗
+        history_at γ back v ∗
+        Φ ()%V
+      )%I with "[HΦ]") as (res) "(%back & -> & #Hhistory_at & HΦ)".
+      { iInv "Hinv" as "(:inv_inner =1)".
+        wp_faa.
+
+        iMod (history_update v with "Hhistory_auth") as "(History_auth & #Hhistory_at)".
+        iEval (rewrite Hhist1) in "Hhistory_at".
+
+        iMod "HΦ" as "(%vs & (:model) & _ & HΦ)".
+        iDestruct (model_agree with "Hmodel₁ Hmodel₂") as %Hvs.
+        iMod (model_update (vs ++ [v]) with "Hmodel₁ Hmodel₂") as "(Hmodel₁ & Hmodel₂)".
+        iMod ("HΦ" with "Hmodel₁ [//]") as "$".
+
+        destruct_decide (front1 ≤ back1) as Hback1.
+
+        - rewrite Nat.max_r //.
+
+          iMod (tokens_update with "Htokens_auth") as "(Htokens_auth & Htokens_at)".
+          iDestruct (big_sepL_seq_snoc_2 with "Hpast [$Htokens_at]") as "Hpast".
+
+          iSplitL.
+          { iExists front1, (S back1). iFrame.
+            simpl_length.
+            rewrite Hvs drop_app_le; first lia.
+            rewrite Nat.max_r; first lia.
+            assert (front1 - S back1 = 0) as -> by lia.
+            iSteps.
+          }
+          iSteps.
+
+        - rewrite Nat.max_l; first lia.
+          rewrite (nil_length_inv vs).
+          { rewrite Hvs length_drop. lia. }
+          assert (front1 - back1 = S (front1 - S back1)) as ->; first lia.
+          destruct (Nat.lt_exists_pred 0 (front1 - back1)) as (δ & ? & _); first lia.
+          iDestruct (big_sepL_seq_cons_1 with "Hwaiters") as "((%Ψ & #Hconsumers_at & HΨ) & Hwaiters)".
+
+          iMod "HΨ" as "(% & Hmodel₁ & _ & HΨ)".
+          iDestruct (model_agree with "Hmodel₁ Hmodel₂") as %->.
+          iMod (model_update [] with "Hmodel₁ Hmodel₂") as "(Hmodel₁ & Hmodel₂)".
+          iMod ("HΨ" with "[$Hmodel₁ //]") as "HΨ".
+
+          iDestruct (big_sepL_seq_snoc_2 with "Hpast [HΨ]") as "Hpast"; first iSteps.
+
+          iSplitL.
+          { iFrame.
+            rewrite skipn_all2 length_app /=; first lia.
+            rewrite Nat.max_l; first lia.
+            iSteps.
+          }
+          iSteps.
+      }
+
+      wp_load.
+
+      awp_apply (inf_array_set_spec with "Hdata_inv") without "HΦ"; first lia.
+      iInv "Hinv" as "(:inv_inner =2)".
+      iAaccIntro with "Hdata_model"; first auto with iFrame. iIntros "Hdata_model !>".
+      iSplitL.
+      { repeat iExists _.
+        rewrite Nat2Z.id -(fn_compose_insert _ _ _ (Something v)).
+        iSteps.
+        rewrite function.fn_lookup_insert.
+        case_decide; first subst; iSteps.
+      }
+      iSteps.
+    Qed.
+
+    #[local] Lemma inf_mpmc_queue_1_pop_0_spec t γ front Ψ :
+      {{{
+        inv' t γ ∗
+        consumers_at γ front Ψ ∗
+        tokens_pending γ front
+      }}}
+        inf_mpmc_queue_1_pop_0 #t #front
+      {{{ v,
+        RET v;
+        Ψ v
+      }}}.
+    Proof.
+      iIntros "%Φ ((:inv') & #Hconsumers_at & Htokens_pending) HΦ".
+
+      iLöb as "HLöb".
+
+      wp_rec credit:"H£". wp_load.
+
+      awp_apply (inf_array_get_spec with "Hdata_inv") without "Htokens_pending H£ HΦ"; first lia.
+      iInv "Hinv" as "(:inv_inner =1)".
+      iAaccIntro with "Hdata_model"; first auto with iFrame. iIntros "Hdata_model".
+      iAssert (▷ slot_model γ front (slots1 front))%I with "[Hslots]" as "#>Hslot"; first iSteps.
+      iSplitL. { iFrameSteps. }
+      iIntros "!> _ (Htokens_pending & H£ & HΦ) {%}".
+
+      rewrite Nat2Z.id /=. destruct (slots1 front) as [| | v].
+
+      - iStep 8.
+        wp_apply ("HLöb" with "Htokens_pending HΦ").
+
+      - iDestruct (tokens_pending_done with "Htokens_pending Hslot") as %[].
+
+      - wp_load.
+
+        awp_apply (inf_array_set_spec with "Hdata_inv") without "H£"; first lia.
+        iInv "Hinv" as "(:inv_inner =2)".
+        iAaccIntro with "Hdata_model"; first auto with iFrame. iIntros "Hdata_model".
+        iDestruct (history_at_valid with "Hhistory_auth Hslot") as %Hhist2_lookup.
+        opose proof* lookup_lt_Some as Hfront; first done.
+        iDestruct (big_sepL_seq_lookup_acc' front with "Hpast") as "([>Htokens_pending_ | (%Ψ_ & Hconsumers_at_ & [>Htokens_done | (%v_ & >Hhistory_at & HΨ)])] & Hpast)"; first lia.
+        { iDestruct (tokens_pending_exclusive with "Htokens_pending Htokens_pending_") as %[]. }
+        { iDestruct (tokens_pending_done with "Htokens_pending Htokens_done") as %[]. }
+        iDestruct (history_at_agree with "Hslot Hhistory_at") as %<-.
+        iDestruct (consumers_at_agree with "Hconsumers_at Hconsumers_at_ HΨ") as "HΨ".
+        iMod (tokens_pending_update with "Htokens_pending") as "#Htokens_done".
+        iDestruct ("Hpast" with "[]") as "Hpast"; first iSteps.
+        iSplitR "HΨ HΦ".
+        { rewrite Nat2Z.id -(fn_compose_insert _ _ _ Anything).
+          iFrameSteps.
+          rewrite function.fn_lookup_insert.
+          case_decide; first subst; iSteps.
+        }
+        iIntros "!> _ H£ {%}".
+
+        iMod (lc_fupd_elim_later with "H£ HΨ") as "HΨ".
+        iSteps.
+    Qed.
+    Lemma inf_mpmc_queue_1_pop_spec t γ ι :
+      <<<
+        inf_mpmc_queue_1_inv t γ ι
+      | ∀∀ vs,
+        inf_mpmc_queue_1_model γ vs
+      >>>
+        inf_mpmc_queue_1_pop #t @ ↑ι
+      <<<
+        ∃∃ v vs',
+        ⌜vs = v :: vs'⌝ ∗
+        inf_mpmc_queue_1_model γ vs'
+      | RET v;
+        True
+      >>>.
+    Proof.
+      iIntros "%Φ (:inv) HΦ".
+
+      wp_rec. wp_pures.
+
+      wp_bind (FAA _ _).
+      wp_apply (wp_wand (λ res,
+        ∃ front,
+        ⌜res = #front⌝ ∗
+        consumers_at γ front Φ ∗
+        tokens_pending γ front
+      )%I with "[HΦ]") as (res) "(%front & -> & Hconsumers_at & Htokens_pending)".
+      { iInv "Hinv" as "(:inv_inner)".
+        wp_faa.
+        destruct_decide (front < back) as Hfront1.
+
+        - rewrite Nat.max_r; first lia.
+          destruct (lookup_lt_is_Some_2 hist front) as (v & Hhist_lookup); first lia.
+          erewrite drop_S; last done.
+
+          iDestruct (history_at_get with "Hhistory_auth") as "#Hhistory_at"; first done.
+          iDestruct (big_sepL_seq_lookup_acc front with "Hpast") as "([$ | (%Ψ & Hconsumers_at & _)] & Hpast)"; first lia; last first.
+          { iDestruct (consumers_at_valid with "Hconsumers_auth Hconsumers_at") as %?. lia. }
+          iMod (consumers_update Φ with "Hconsumers_auth") as "(Hconsumers_auth & #Hconsumers_at)".
+
+          iMod "HΦ" as "(%vs & (:model) & _ & HΦ)".
+          iDestruct (model_agree with "Hmodel₁ Hmodel₂") as %->.
+          iMod (model_update (drop (S front) hist) with "Hmodel₁ Hmodel₂") as "(Hmodel₁ & Hmodel₂)".
+          iMod ("HΦ" with "[$Hmodel₁ //] [//]") as "HΦ".
+
+          iSplitL.
+          { iFrameSteps.
+            rewrite Nat.max_r //.
+            assert (S front - back = 0) as -> by lia.
+            iSteps.
+          }
+          iSteps.
+
+        - rewrite Nat.max_l; first lia.
+
+          iMod (consumers_update Φ with "Hconsumers_auth") as "(Hconsumers_auth & #Hconsumers_at)".
+          iMod (tokens_update with "Htokens_auth") as "(Htokens_auth & $)".
+          iDestruct (big_sepL_seq_snoc_2 with "Hwaiters [HΦ]") as "Hwaiters".
+          { rewrite -Nat.le_add_sub; first lia.
+            iSteps. rewrite /consumer_au. iAuIntro.
+            iApply (aacc_aupd_commit with "HΦ"); first done. iIntros "%vs (:model)".
+            iAaccIntro with "Hmodel₁"; iSteps.
+          }
+          rewrite -Nat.sub_succ_l; first lia.
+
+          iSplitL.
+          { iFrameSteps.
+            rewrite !skipn_all2; [lia.. |].
+            rewrite Nat.max_l; first lia.
+            iSteps.
+          }
+          iSteps.
+      }
+
+      wp_smart_apply (inf_mpmc_queue_1_pop_0_spec with "[$Hconsumers_at $Htokens_pending]"); iSteps.
+    Qed.
+  End inf_mpmc_queue_1_G.
+
+  #[global] Opaque inf_mpmc_queue_1_inv.
+  #[global] Opaque inf_mpmc_queue_1_model.
+End base.
+
+From zoo_saturn Require
+  inf_mpmc_queue_1__opaque.
+
 Section inf_mpmc_queue_1_G.
   Context `{inf_mpmc_queue_1_G : InfMpmcQueue1G Σ}.
 
-  Implicit Types Ψ : val → iProp Σ.
+  Implicit Types 𝑡 : location.
+  Implicit Types t : val.
 
-  Record metadata := {
-    metadata_data : val ;
-    metadata_inv : namespace ;
-    metadata_model : gname ;
-    metadata_history : gname ;
-    metadata_consumers : gname ;
-    metadata_tokens : gname ;
-  }.
-  Implicit Types γ : metadata.
-
-  #[local] Instance metadata_eq_dec : EqDecision metadata :=
-    ltac:(solve_decision).
-  #[local] Instance metadata_countable :
-    Countable metadata.
-  Proof.
-    solve_countable.
-  Qed.
-
-  #[local] Definition model₁' γ_model vs :=
-    twins_twin1 γ_model (DfracOwn 1) vs.
-  #[local] Definition model₁ γ :=
-    model₁' γ.(metadata_model).
-  #[local] Definition model₂' γ_model vs :=
-    twins_twin2 γ_model vs.
-  #[local] Definition model₂ γ :=
-    model₂' γ.(metadata_model).
-
-  #[local] Definition history_auth' γ_history hist :=
-    mono_list_auth γ_history (DfracOwn 1) hist.
-  #[local] Definition history_auth γ :=
-    history_auth' γ.(metadata_history).
-  #[local] Definition history_at γ i v :=
-    mono_list_at γ.(metadata_history) i v.
-
-  #[local] Definition consumers_auth' γ_consumers i : iProp Σ :=
-    ∃ ηs,
-    mono_list_auth γ_consumers (DfracOwn 1) ηs ∗
-    ⌜length ηs = i⌝.
-  #[local] Definition consumers_auth γ i :=
-    consumers_auth' γ.(metadata_consumers) i.
-  #[local] Instance : CustomIpatFormat "consumers_auth" :=
-    " ( %ηs{} &
-        Hauth{} &
-        %Hηs{}
-      )
-    ".
-  #[local] Definition consumers_at γ i Ψ : iProp Σ :=
-    ∃ η,
-    mono_list_at γ.(metadata_consumers) i η ∗
-    saved_pred η Ψ.
-  #[local] Instance : CustomIpatFormat "consumers_at" :=
-    " ( %η{} &
-        Hat{} &
-        HΨ{}
-      )
-    ".
-  #[local] Definition consumers_lb γ i : iProp Σ :=
-    ∃ ηs,
-    ⌜length ηs = i⌝ ∗
-    mono_list_lb γ.(metadata_consumers) ηs.
-  #[local] Instance : CustomIpatFormat "consumers_lb" :=
-    " ( %ηs{} &
-        %Hηs{} &
-        Hlb{}
-      )
-    ".
-
-  #[local] Definition tokens_auth' γ_tokens i : iProp Σ :=
-    ∃ ηs,
-    mono_list_auth γ_tokens (DfracOwn 1) ηs ∗
-    ⌜length ηs = i⌝.
-  #[local] Definition tokens_auth γ i :=
-    tokens_auth' γ.(metadata_tokens) i.
-  #[local] Instance : CustomIpatFormat "tokens_auth" :=
-    " ( %ηs{} &
-        Hauth{} &
-        %Hηs{}
-      )
-    ".
-  #[local] Definition tokens_pending γ i : iProp Σ :=
-    ∃ η,
-    mono_list_at γ.(metadata_tokens) i η ∗
-    oneshot_pending η (DfracOwn 1) ().
-  #[local] Instance : CustomIpatFormat "tokens_pending" :=
-    " ( %η{} &
-        Hat{} &
-        Hpending{}
-      )
-    ".
-  #[local] Definition tokens_done γ i : iProp Σ :=
-    ∃ η,
-    mono_list_at γ.(metadata_tokens) i η ∗
-    oneshot_shot η ().
-  #[local] Instance : CustomIpatFormat "tokens_done" :=
-    " ( %η{} &
-        Hat{} &
-        Hshot{}
-      )
-    ".
-
-  #[local] Definition consumer_au γ Ψ : iProp Σ :=
-    AU <{
-      ∃∃ vs,
-      model₁ γ vs
-    }> @ ⊤ ∖ ↑γ.(metadata_inv), ∅ <{
-      ∀∀ v vs',
-      ⌜vs = v :: vs'⌝ ∗
-      model₁ γ vs'
-    , COMM
-      Ψ v
-    }>.
-
-  #[local] Definition slot_model γ i slot : iProp Σ :=
-    match slot with
-    | Something v =>
-        history_at γ i v
-    | Anything =>
-        tokens_done γ i
-    | Nothing =>
-        True
-    end.
-  #[local] Definition inv_inner l γ : iProp Σ :=
-    ∃ front back hist slots,
-    l.[front] ↦ #front ∗
-    l.[back] ↦ #back ∗
-    inf_array_model γ.(metadata_data) (optional_to_val ∘ slots) ∗
-    history_auth γ hist ∗
-    ⌜length hist = back⌝ ∗
-    model₂ γ (drop front hist) ∗
-    consumers_auth γ front ∗
-    tokens_auth γ (front `max` back) ∗
-    ( [∗ list] i ∈ seq 0 back,
-        tokens_pending γ i
-      ∨ ∃ Ψ,
-        consumers_at γ i Ψ ∗
-        ( tokens_done γ i
-        ∨ ∃ v,
-          history_at γ i v ∗
-          Ψ v
-        )
-    ) ∗
-    ( [∗ list] i ∈ seq back (front - back),
-      ∃ Ψ,
-      consumers_at γ i Ψ ∗
-      consumer_au γ Ψ
-    ) ∗
-    (∀ i, slot_model γ i (slots i)).
-  #[local] Instance : CustomIpatFormat "inv_inner" :=
-    " ( %front{} &
-        %back{} &
-        %hist{} &
-        %slots{} &
-        Hl_front &
-        Hl_back &
-        >Hdata_model &
-        >Hhistory_auth &
-        >%Hhist{} &
-        Hmodel₂ &
-        Hconsumers_auth &
-        Htokens_auth &
-        Hpast &
-        Hwaiters &
-        Hslots
-      )
-    ".
-  Definition inv' l γ : iProp Σ :=
-    meta l nroot γ ∗
-    l.[data] ↦□ γ.(metadata_data) ∗
-    inf_array_inv γ.(metadata_data) ∗
-    inv γ.(metadata_inv) (inv_inner l γ).
-  #[local] Instance : CustomIpatFormat "inv'" :=
-    " ( #Hmeta &
-        #Hl_data &
-        #Hdata_inv &
-        #Hinv
-      )
-    ".
   Definition inf_mpmc_queue_1_inv t ι : iProp Σ :=
-    ∃ l γ,
-    ⌜t = #l⌝ ∗
-    ⌜ι = γ.(metadata_inv)⌝ ∗
-    inv' l γ.
+    ∃ 𝑡 γ,
+    ⌜t = #𝑡⌝ ∗
+    meta 𝑡 nroot γ ∗
+    base.inf_mpmc_queue_1_inv 𝑡 γ ι.
   #[local] Instance : CustomIpatFormat "inv" :=
-    " ( %l &
-        %γ &
-        -> &
-        -> &
-        (:inv')
+    " ( %𝑡{} &
+        %γ{} &
+        {%Heq{};->} &
+        #Hmeta{_{}} &
+        Hinv{_{}}
       )
     ".
 
   Definition inf_mpmc_queue_1_model t vs : iProp Σ :=
-    ∃ l γ,
-    ⌜t = #l⌝ ∗
-    meta l nroot γ ∗
-    model₁ γ vs.
+    ∃ 𝑡 γ,
+    ⌜t = #𝑡⌝ ∗
+    meta 𝑡 nroot γ ∗
+    base.inf_mpmc_queue_1_model γ vs.
   #[local] Instance : CustomIpatFormat "model" :=
-    " ( %l{;_} &
-        %γ{;_} &
-        %Heq{} &
-        Hmeta_{} &
-        Hmodel₁{_{}}
+    " ( %𝑡{} &
+        %γ{} &
+        {%Heq{};->} &
+        Hmeta{_{}} &
+        Hmodel{_{}}
       )
     ".
 
-  #[local] Instance tokens_pending_timeless γ i :
-    Timeless (tokens_pending γ i).
-  Proof.
-    apply _.
-  Qed.
-  #[local] Instance tokens_done_timeless γ i :
-    Timeless (tokens_done γ i).
-  Proof.
-    apply _.
-  Qed.
-  #[local] Instance slot_model_timeless γ i slot :
-    Timeless (slot_model γ i slot).
-  Proof.
-    rewrite /slot_model. apply _.
-  Qed.
   #[global] Instance inf_mpmc_queue_1_model_timeless t vs :
     Timeless (inf_mpmc_queue_1_model t vs).
   Proof.
     apply _.
   Qed.
 
-  #[local] Instance consumers_at_persistent γ i Ψ :
-    Persistent (consumers_at γ i Ψ).
-  Proof.
-    apply _.
-  Qed.
-  #[local] Instance consumers_lb_persistent γ i :
-    Persistent (consumers_lb γ i).
-  Proof.
-    apply _.
-  Qed.
-  #[local] Instance tokens_done_persistent γ i :
-    Persistent (tokens_done γ i).
-  Proof.
-    apply _.
-  Qed.
-  #[local] Instance slot_model_persistent γ i slot :
-    Persistent (slot_model γ i slot).
-  Proof.
-    rewrite /slot_model. apply _.
-  Qed.
   #[global] Instance inf_mpmc_queue_1_inv_persistent t ι :
     Persistent (inf_mpmc_queue_1_inv t ι).
   Proof.
     apply _.
   Qed.
-
-  #[local] Lemma model_alloc :
-    ⊢ |==>
-      ∃ γ_model,
-      model₁' γ_model [] ∗
-      model₂' γ_model [].
-  Proof.
-    apply twins_alloc'.
-  Qed.
-  #[local] Lemma model₁_exclusive γ vs1 vs2 :
-    model₁ γ vs1 -∗
-    model₁ γ vs2 -∗
-    False.
-  Proof.
-    apply twins_twin1_exclusive.
-  Qed.
-  #[local] Lemma model_agree γ vs1 vs2 :
-    model₁ γ vs1 -∗
-    model₂ γ vs2 -∗
-    ⌜vs1 = vs2⌝.
-  Proof.
-    apply: twins_agree_L.
-  Qed.
-  #[local] Lemma model_update {γ vs1 vs2} vs :
-    model₁ γ vs1 -∗
-    model₂ γ vs2 ==∗
-      model₁ γ vs ∗
-      model₂ γ vs.
-  Proof.
-    apply twins_update.
-  Qed.
-
-  #[local] Lemma history_alloc :
-    ⊢ |==>
-      ∃ γ_history,
-      history_auth' γ_history [].
-  Proof.
-    apply mono_list_alloc.
-  Qed.
-  #[local] Lemma history_at_valid γ hist i v :
-    history_auth γ hist -∗
-    history_at γ i v -∗
-    ⌜hist !! i = Some v⌝.
-  Proof.
-    apply mono_list_at_valid.
-  Qed.
-  #[local] Lemma history_at_agree γ i v1 v2 :
-    history_at γ i v1 -∗
-    history_at γ i v2 -∗
-    ⌜v1 = v2⌝.
-  Proof.
-    apply mono_list_at_agree.
-  Qed.
-  #[local] Lemma history_at_get {γ hist} i v :
-    hist !! i = Some v →
-    history_auth γ hist ⊢
-    history_at γ i v.
-  Proof.
-    apply mono_list_at_get.
-  Qed.
-  #[local] Lemma history_update {γ hist} v :
-    history_auth γ hist ⊢ |==>
-      history_auth γ (hist ++ [v]) ∗
-      history_at γ (length hist) v.
-  Proof.
-    iIntros "Hhistory_auth".
-    iMod (mono_list_update_snoc v with "Hhistory_auth") as "Hhistory_auth".
-    iDestruct (mono_list_at_get with "Hhistory_auth") as "#Hhistory_at".
-    { rewrite list_lookup_middle //. }
-    iSteps.
-  Qed.
-
-  #[local] Lemma consumers_alloc :
-    ⊢ |==>
-      ∃ γ_consumers,
-      consumers_auth' γ_consumers 0.
-  Proof.
-    iMod mono_list_alloc as "(%γ_consumers & Hauth)".
-    iExists _, []. iSteps.
-  Qed.
-  #[local] Lemma consumers_at_valid γ i j Ψ :
-    consumers_auth γ i -∗
-    consumers_at γ j Ψ -∗
-    ⌜j < i⌝.
-  Proof.
-    iIntros "(:consumers_auth) (:consumers_at)".
-    iDestruct (mono_list_at_valid with "Hauth Hat") as %?Hj%lookup_lt_Some.
-    iSteps.
-  Qed.
-  #[local] Lemma consumers_at_agree γ i Ψ1 Ψ2 v :
-    consumers_at γ i Ψ1 -∗
-    ▷ consumers_at γ i Ψ2 -∗
-    ▷ Ψ2 v -∗
-    ▷^2 Ψ1 v.
-  Proof.
-    iIntros "(:consumers_at =1) (:consumers_at =2) HΨ !>".
-    iDestruct (mono_list_at_agree with "Hat1 Hat2") as %<-.
-    iDestruct (saved_pred_agree v with "HΨ1 HΨ2") as "Heq".
-    iModIntro. iRewrite "Heq". iSteps.
-  Qed.
-  #[local] Lemma consumers_lb_valid γ i j :
-    consumers_auth γ i -∗
-    consumers_lb γ j -∗
-    ⌜j ≤ i⌝.
-  Proof.
-    iIntros "(:consumers_auth =1) (:consumers_lb =2)".
-    iDestruct (mono_list_lb_valid with "Hauth1 Hlb2") as %?%prefix_length.
-    iSteps.
-  Qed.
-  #[local] Lemma consumers_lb_get γ i :
-    consumers_auth γ i ⊢
-    consumers_lb γ i.
-  Proof.
-    iIntros "(:consumers_auth)".
-    iDestruct (mono_list_lb_get with "Hauth") as "Hlb".
-    iSteps.
-  Qed.
-  #[local] Lemma consumers_update {γ i} Ψ :
-    consumers_auth γ i ⊢ |==>
-      consumers_auth γ (S i) ∗
-      consumers_at γ i Ψ.
-  Proof.
-    iIntros "(:consumers_auth)".
-    iMod (saved_pred_alloc Ψ) as "(%η & HΨ)".
-    iMod (mono_list_update_snoc with "Hauth") as "Hauth".
-    iDestruct (mono_list_at_get with "Hauth") as "#Hat".
-    { rewrite list_lookup_middle //. }
-    iFrame. simpl_length. iSteps.
-  Qed.
-
-  #[local] Lemma tokens_alloc :
-    ⊢ |==>
-      ∃ γ_tokens,
-      tokens_auth' γ_tokens 0.
-  Proof.
-    iMod mono_list_alloc as "(%γ_tokens & Hauth)".
-    iExists _, []. iSteps.
-  Qed.
-  #[local] Lemma tokens_pending_exclusive γ i :
-    tokens_pending γ i -∗
-    tokens_pending γ i -∗
-    False.
-  Proof.
-    iIntros "(:tokens_pending =1) (:tokens_pending =2)".
-    iDestruct (mono_list_at_agree with "Hat1 Hat2") as %<-.
-    iApply (oneshot_pending_exclusive with "Hpending1 Hpending2").
-  Qed.
-  #[local] Lemma tokens_pending_done γ i :
-    tokens_pending γ i -∗
-    tokens_done γ i -∗
-    False.
-  Proof.
-    iIntros "(:tokens_pending =1) (:tokens_done =2)".
-    iDestruct (mono_list_at_agree with "Hat1 Hat2") as %<-.
-    iApply (oneshot_pending_shot with "Hpending1 Hshot2").
-  Qed.
-  #[local] Lemma tokens_update {γ} i :
-    tokens_auth γ i ⊢ |==>
-      tokens_auth γ (S i) ∗
-      tokens_pending γ i.
-  Proof.
-    iIntros "(:tokens_auth)".
-    iMod oneshot_alloc as "(%η & Hpending)".
-    iMod (mono_list_update_snoc with "Hauth") as "Hauth".
-    iDestruct (mono_list_at_get with "Hauth") as "#Hat".
-    { rewrite list_lookup_middle //. }
-    iFrame. simpl_length. iSteps.
-  Qed.
-  #[local] Lemma tokens_pending_update γ i :
-    tokens_pending γ i ⊢ |==>
-    tokens_done γ i.
-  Proof.
-    iIntros "(:tokens_pending)".
-    iMod (oneshot_update_shot with "Hpending") as "Hshot".
-    iSteps.
-  Qed.
-
-  Opaque consumers_auth'.
-  Opaque consumers_at.
-  Opaque consumers_lb.
-  Opaque tokens_auth'.
-  Opaque tokens_pending.
-  Opaque tokens_done.
 
   Lemma inf_mpmc_queue_1_model_exclusive t vs1 vs2 :
     inf_mpmc_queue_1_model t vs1 -∗
@@ -530,7 +949,7 @@ Section inf_mpmc_queue_1_G.
   Proof.
     iIntros "(:model =1) (:model =2)". simplify.
     iDestruct (meta_agree with "Hmeta_1 Hmeta_2") as %->.
-    iApply (model₁_exclusive with "Hmodel₁_1 Hmodel₁_2").
+    iApply (base.inf_mpmc_queue_1_model_exclusive with "Hmodel_1 Hmodel_2").
   Qed.
 
   Lemma inf_mpmc_queue_1_create_spec ι :
@@ -546,29 +965,10 @@ Section inf_mpmc_queue_1_G.
   Proof.
     iIntros "%Φ _ HΦ".
 
-    wp_rec.
-    wp_apply (inf_array_create_spec with "[//]") as (data) "(#Hdata_inv & Hdata_model)".
-    wp_block l as "Hmeta" "(Hl_data & Hl_front & Hl_back & _)".
-    iMod (pointsto_persist with "Hl_data") as "#Hl_data".
-
-    iMod model_alloc as "(%γ_model & Hmodel₁ & Hmodel₂)".
-    iMod history_alloc as "(%γ_history & Hhistory_auth)".
-    iMod consumers_alloc as "(%γ_consumers & Hconsumers_auth)".
-    iMod tokens_alloc as "(%γ_tokens & Htokens_auth)".
-
-    pose γ := {|
-      metadata_data := data ;
-      metadata_inv := ι ;
-      metadata_model := γ_model ;
-      metadata_history := γ_history ;
-      metadata_consumers := γ_consumers ;
-      metadata_tokens := γ_tokens ;
-    |}.
-    iMod (meta_set γ with "Hmeta") as "#Hmeta"; first done.
-
-    iApply "HΦ".
-    iSplitR "Hmodel₁"; last iSteps.
-    iExists l, γ. iSteps. iExists (λ _, Nothing). iSteps.
+    iApply wp_fupd.
+    wp_apply (base.inf_mpmc_queue_1_create_spec with "[//]") as (𝑡 γ) "(Hmeta & Hinv & Hmodel)".
+    iMod (meta_set γ with "Hmeta"); first done.
+    iSteps.
   Qed.
 
   Lemma inf_mpmc_queue_1_size_spec t ι :
@@ -586,78 +986,11 @@ Section inf_mpmc_queue_1_G.
   Proof.
     iIntros "%Φ (:inv) HΦ".
 
-    iLöb as "HLöb".
-
-    wp_rec.
-
-    wp_bind (_.{front})%E.
-    iInv "Hinv" as "(:inv_inner =1)".
-    wp_load.
-    iDestruct (consumers_lb_get with "Hconsumers_auth") as "#Hconsumers_lb1".
-    iSplitR "HΦ". { iFrameSteps. }
-    iIntros "!> {%}".
-
-    wp_smart_apply (typed_prophet1_wp_proph prophet with "[//]") as (pid proph) "Hproph".
-    wp_pures.
-
-    wp_bind (_.{back})%E.
-    iInv "Hinv" as "(:inv_inner =2)".
-    wp_load.
-    destruct_decide (proph = front1) as -> | Hproph.
-
-    - destruct_decide (front2 = front1) as -> | ?.
-
-      + iMod "HΦ" as "(%vs & (:model) & _ & HΦ)". injection Heq as <-.
-        iDestruct (meta_agree with "Hmeta Hmeta_") as %<-. iClear "Hmeta_".
-        iDestruct (model_agree with "Hmodel₁ Hmodel₂") as %->.
-        iMod ("HΦ" with "[Hmodel₁] [//]") as "HΦ"; first iSteps.
-
-        iSplitR "Hproph HΦ". { iFrameSteps. }
-        iModIntro. clear- Hhist2.
-
-        wp_pures.
-
-        wp_bind (_.{front})%E.
-        iInv "Hinv" as "(:inv_inner =3)".
-        wp_load.
-        iSplitR "Hproph HΦ". { iFrameSteps. }
-        iModIntro. clear- Hhist2.
-
-        wp_smart_apply (typed_prophet1_wp_resolve with "Hproph"); [done.. |].
-        iSteps.
-        rewrite length_drop Hhist2 Z2Nat.inj_sub; first lia.
-        rewrite !Nat2Z.id //.
-
-      + iDestruct (consumers_lb_valid with "Hconsumers_auth Hconsumers_lb1") as %?.
-        iDestruct (consumers_lb_get with "Hconsumers_auth") as "#Hconsumers_lb2".
-        iSplitR "Hproph HΦ". { iFrameSteps. }
-        iModIntro.
-
-        wp_pures.
-
-        wp_bind (_.{front})%E.
-        iInv "Hinv" as "(:inv_inner =3)".
-        wp_load.
-        iDestruct (consumers_lb_valid with "Hconsumers_auth Hconsumers_lb2") as %?.
-        iSplitR "Hproph HΦ". { iFrameSteps. }
-        iModIntro.
-
-        wp_smart_apply (typed_prophet1_wp_resolve with "Hproph"); [done.. |].
-        iSteps.
-
-    - iSplitR "Hproph HΦ". { iFrameSteps. }
-      iModIntro. clear- Hproph.
-
-      wp_pures.
-
-      wp_bind (_.{front})%E.
-      iInv "Hinv" as "(:inv_inner =3)".
-      wp_load.
-      iSplitR "Hproph HΦ". { iFrameSteps. }
-      iModIntro. clear- Hproph.
-
-      wp_smart_apply (typed_prophet1_wp_resolve with "Hproph"); [done.. |].
-      iSteps.
+    awp_apply (base.inf_mpmc_queue_1_size_spec with "[$]").
+    { iApply (aacc_aupd_commit with "HΦ"); first done. iIntros "%vs (:model =1)". simplify.
+      iDestruct (meta_agree with "Hmeta Hmeta_1") as %<-. iClear "Hmeta_1".
+      iAaccIntro with "Hmodel_1"; iSteps.
+    }
   Qed.
 
   Lemma inf_mpmc_queue_1_is_empty_spec t ι :
@@ -673,14 +1006,13 @@ Section inf_mpmc_queue_1_G.
       True
     >>>.
   Proof.
-    iIntros "%Φ #Hinv HΦ".
+    iIntros "%Φ (:inv) HΦ".
 
-    wp_rec.
-
-    awp_apply (inf_mpmc_queue_1_size_spec with "Hinv").
-    iApply (aacc_aupd_commit with "HΦ"); first done. iIntros "%vs Hmodel".
-    iAaccIntro with "Hmodel"; iSteps.
-    destruct vs; iSteps.
+    awp_apply (base.inf_mpmc_queue_1_is_empty_spec with "[$]").
+    { iApply (aacc_aupd_commit with "HΦ"); first done. iIntros "%vs (:model =1)". simplify.
+      iDestruct (meta_agree with "Hmeta Hmeta_1") as %<-. iClear "Hmeta_1".
+      iAaccIntro with "Hmodel_1"; iSteps.
+    }
   Qed.
 
   Lemma inf_mpmc_queue_1_push_spec t ι v :
@@ -698,139 +1030,13 @@ Section inf_mpmc_queue_1_G.
   Proof.
     iIntros "%Φ (:inv) HΦ".
 
-    wp_rec. wp_pures.
-
-    wp_bind (FAA _ _).
-    wp_apply (wp_wand (λ res,
-      ∃ back,
-      ⌜res = #back⌝ ∗
-      history_at γ back v ∗
-      Φ ()%V
-    )%I with "[HΦ]") as (res) "(%back & -> & #Hhistory_at & HΦ)".
-    { iInv "Hinv" as "(:inv_inner =1)".
-      wp_faa.
-
-      iMod (history_update v with "Hhistory_auth") as "(History_auth & #Hhistory_at)".
-      iEval (rewrite Hhist1) in "Hhistory_at".
-
-      iMod "HΦ" as "(%vs & (:model) & _ & HΦ)". injection Heq as <-.
-      iDestruct (meta_agree with "Hmeta Hmeta_") as %<-. iClear "Hmeta_".
-      iDestruct (model_agree with "Hmodel₁ Hmodel₂") as %Hvs.
-      iMod (model_update (vs ++ [v]) with "Hmodel₁ Hmodel₂") as "(Hmodel₁ & Hmodel₂)".
-      iMod ("HΦ" with "[Hmodel₁] [//]") as "$"; first iSteps.
-
-      destruct_decide (front1 ≤ back1) as Hback1.
-
-      - rewrite Nat.max_r //.
-
-        iMod (tokens_update with "Htokens_auth") as "(Htokens_auth & Htokens_at)".
-        iDestruct (big_sepL_seq_snoc_2 with "Hpast [$Htokens_at]") as "Hpast".
-
-        iSplitL.
-        { iExists front1, (S back1). iFrame.
-          simpl_length.
-          rewrite Hvs drop_app_le; first lia.
-          rewrite Nat.max_r; first lia.
-          assert (front1 - S back1 = 0) as -> by lia.
-          iSteps.
-        }
-        iSteps.
-
-      - rewrite Nat.max_l; first lia.
-        rewrite (nil_length_inv vs).
-        { rewrite Hvs length_drop. lia. }
-        assert (front1 - back1 = S (front1 - S back1)) as ->; first lia.
-        destruct (Nat.lt_exists_pred 0 (front1 - back1)) as (δ & ? & _); first lia.
-        iDestruct (big_sepL_seq_cons_1 with "Hwaiters") as "((%Ψ & #Hconsumers_at & HΨ) & Hwaiters)".
-
-        iMod "HΨ" as "(% & Hmodel₁ & _ & HΨ)".
-        iDestruct (model_agree with "Hmodel₁ Hmodel₂") as %->.
-        iMod (model_update [] with "Hmodel₁ Hmodel₂") as "(Hmodel₁ & Hmodel₂)".
-        iMod ("HΨ" with "[$Hmodel₁ //]") as "HΨ".
-
-        iDestruct (big_sepL_seq_snoc_2 with "Hpast [HΨ]") as "Hpast"; first iSteps.
-
-        iSplitL.
-        { iFrame.
-          rewrite skipn_all2 length_app /=; first lia.
-          rewrite Nat.max_l; first lia.
-          iSteps.
-        }
-        iSteps.
+    awp_apply (base.inf_mpmc_queue_1_push_spec with "[$]").
+    { iApply (aacc_aupd_commit with "HΦ"); first done. iIntros "%vs (:model =1)". simplify.
+      iDestruct (meta_agree with "Hmeta Hmeta_1") as %<-. iClear "Hmeta_1".
+      iAaccIntro with "Hmodel_1"; iSteps.
     }
-
-    wp_load.
-
-    awp_apply (inf_array_set_spec with "Hdata_inv") without "HΦ"; first lia.
-    iInv "Hinv" as "(:inv_inner =2)".
-    iAaccIntro with "Hdata_model"; first auto with iFrame. iIntros "Hdata_model !>".
-    iSplitL.
-    { repeat iExists _.
-      rewrite Nat2Z.id -(fn_compose_insert _ _ _ (Something v)).
-      iSteps.
-      rewrite function.fn_lookup_insert.
-      case_decide; first subst; iSteps.
-    }
-    iSteps.
   Qed.
 
-  #[local] Lemma inf_mpmc_queue_1_pop_0_spec l γ front Ψ :
-    {{{
-      inv' l γ ∗
-      consumers_at γ front Ψ ∗
-      tokens_pending γ front
-    }}}
-      inf_mpmc_queue_1_pop_0 #l #front
-    {{{ v,
-      RET v;
-      Ψ v
-    }}}.
-  Proof.
-    iIntros "%Φ ((:inv') & #Hconsumers_at & Htokens_pending) HΦ".
-
-    iLöb as "HLöb".
-
-    wp_rec credit:"H£". wp_load.
-
-    awp_apply (inf_array_get_spec with "Hdata_inv") without "Htokens_pending H£ HΦ"; first lia.
-    iInv "Hinv" as "(:inv_inner =1)".
-    iAaccIntro with "Hdata_model"; first auto with iFrame. iIntros "Hdata_model".
-    iAssert (▷ slot_model γ front (slots1 front))%I with "[Hslots]" as "#>Hslot"; first iSteps.
-    iSplitL. { iFrameSteps. }
-    iIntros "!> _ (Htokens_pending & H£ & HΦ) {%}".
-
-    rewrite Nat2Z.id /=. destruct (slots1 front) as [| | v].
-
-    - iStep 8.
-      wp_apply ("HLöb" with "Htokens_pending HΦ").
-
-    - iDestruct (tokens_pending_done with "Htokens_pending Hslot") as %[].
-
-    - wp_load.
-
-      awp_apply (inf_array_set_spec with "Hdata_inv") without "H£"; first lia.
-      iInv "Hinv" as "(:inv_inner =2)".
-      iAaccIntro with "Hdata_model"; first auto with iFrame. iIntros "Hdata_model".
-      iDestruct (history_at_valid with "Hhistory_auth Hslot") as %Hhist2_lookup.
-      opose proof* lookup_lt_Some as Hfront; first done.
-      iDestruct (big_sepL_seq_lookup_acc' front with "Hpast") as "([>Htokens_pending_ | (%Ψ_ & Hconsumers_at_ & [>Htokens_done | (%v_ & >Hhistory_at & HΨ)])] & Hpast)"; first lia.
-      { iDestruct (tokens_pending_exclusive with "Htokens_pending Htokens_pending_") as %[]. }
-      { iDestruct (tokens_pending_done with "Htokens_pending Htokens_done") as %[]. }
-      iDestruct (history_at_agree with "Hslot Hhistory_at") as %<-.
-      iDestruct (consumers_at_agree with "Hconsumers_at Hconsumers_at_ HΨ") as "HΨ".
-      iMod (tokens_pending_update with "Htokens_pending") as "#Htokens_done".
-      iDestruct ("Hpast" with "[]") as "Hpast"; first iSteps.
-      iSplitR "HΨ HΦ".
-      { rewrite Nat2Z.id -(fn_compose_insert _ _ _ Anything).
-        iFrameSteps.
-        rewrite function.fn_lookup_insert.
-        case_decide; first subst; iSteps.
-      }
-      iIntros "!> _ H£ {%}".
-
-      iMod (lc_fupd_elim_later with "H£ HΨ") as "HΨ".
-      iSteps.
-  Qed.
   Lemma inf_mpmc_queue_1_pop_spec t ι :
     <<<
       inf_mpmc_queue_1_inv t ι
@@ -848,70 +1054,13 @@ Section inf_mpmc_queue_1_G.
   Proof.
     iIntros "%Φ (:inv) HΦ".
 
-    wp_rec. wp_pures.
-
-    wp_bind (FAA _ _).
-    wp_apply (wp_wand (λ res,
-      ∃ front,
-      ⌜res = #front⌝ ∗
-      consumers_at γ front Φ ∗
-      tokens_pending γ front
-    )%I with "[HΦ]") as (res) "(%front & -> & Hconsumers_at & Htokens_pending)".
-    { iInv "Hinv" as "(:inv_inner)".
-      wp_faa.
-      destruct_decide (front < back) as Hfront1.
-
-      - rewrite Nat.max_r; first lia.
-        destruct (lookup_lt_is_Some_2 hist front) as (v & Hhist_lookup); first lia.
-        erewrite drop_S; last done.
-
-        iDestruct (history_at_get with "Hhistory_auth") as "#Hhistory_at"; first done.
-        iDestruct (big_sepL_seq_lookup_acc front with "Hpast") as "([$ | (%Ψ & Hconsumers_at & _)] & Hpast)"; first lia; last first.
-        { iDestruct (consumers_at_valid with "Hconsumers_auth Hconsumers_at") as %?. lia. }
-        iMod (consumers_update Φ with "Hconsumers_auth") as "(Hconsumers_auth & #Hconsumers_at)".
-
-        iMod "HΦ" as "(%vs & (:model) & _ & HΦ)". injection Heq as <-.
-        iDestruct (meta_agree with "Hmeta Hmeta_") as %<-. iClear "Hmeta_".
-        iDestruct (model_agree with "Hmodel₁ Hmodel₂") as %->.
-        iMod (model_update (drop (S front) hist) with "Hmodel₁ Hmodel₂") as "(Hmodel₁ & Hmodel₂)".
-        iMod ("HΦ" with "[Hmodel₁] [//]") as "HΦ"; first iSteps.
-
-        iSplitL.
-        { iFrameSteps.
-          rewrite Nat.max_r //.
-          assert (S front - back = 0) as -> by lia.
-          iSteps.
-        }
-        iSteps.
-
-      - rewrite Nat.max_l; first lia.
-
-        iMod (consumers_update Φ with "Hconsumers_auth") as "(Hconsumers_auth & #Hconsumers_at)".
-        iMod (tokens_update with "Htokens_auth") as "(Htokens_auth & $)".
-        iDestruct (big_sepL_seq_snoc_2 with "Hwaiters [HΦ]") as "Hwaiters".
-        { rewrite -Nat.le_add_sub; first lia.
-          iSteps. rewrite /consumer_au. iAuIntro.
-          iApply (aacc_aupd_commit with "HΦ"); first done. iIntros "%vs (:model)". injection Heq as <-.
-          iDestruct (meta_agree with "Hmeta Hmeta_") as %<-. iClear "Hmeta_".
-          iAaccIntro with "Hmodel₁"; iSteps.
-        }
-        rewrite -Nat.sub_succ_l; first lia.
-
-        iSplitL.
-        { iFrameSteps.
-          rewrite !skipn_all2; [lia.. |].
-          rewrite Nat.max_l; first lia.
-          iSteps.
-        }
-        iSteps.
+    awp_apply (base.inf_mpmc_queue_1_pop_spec with "[$]").
+    { iApply (aacc_aupd_commit with "HΦ"); first done. iIntros "%vs (:model =1)". simplify.
+      iDestruct (meta_agree with "Hmeta Hmeta_1") as %<-. iClear "Hmeta_1".
+      iAaccIntro with "Hmodel_1"; iSteps.
     }
-
-    wp_smart_apply (inf_mpmc_queue_1_pop_0_spec with "[$Hconsumers_at $Htokens_pending]"); iSteps.
   Qed.
 End inf_mpmc_queue_1_G.
-
-From zoo_saturn Require
-  inf_mpmc_queue_1__opaque.
 
 #[global] Opaque inf_mpmc_queue_1_inv.
 #[global] Opaque inf_mpmc_queue_1_model.
